AwsCryptographicMaterialProviders/dafny/AwsCryptographyKeyStore/src/Structure.dfy
@@ -462,6 +462,10 @@ module {:options "/functionSyntax:4" } Structure {
     ensures BRANCH_KEY_ACTIVE_VERSION_FIELD !in output
     ensures output[KMS_FIELD] == kmsKeyArn
     ensures output[TABLE_FIELD] == logicalKeyStoreName
+    ensures
+      match hierachyVersion
+      case v1 => output[HIERARCHY_VERSION] == HIERARCHY_VERSION_VALUE_1
+      case v2 => output[HIERARCHY_VERSION] == HIERARCHY_VERSION_VALUE_2
     ensures forall k <- customEncryptionContext
               ::
                 && ENCRYPTION_CONTEXT_PREFIX + k in output
